SystemF2Effect: fixing closedT goals in preservation SfRegionNew
Ignore-this: bef9b3ac945f30aa31a0484b26048607

darcs-hash:20130213070028-08f32-24f2f2b48a29c24d885dbbba628e430870a99fc4

devel/Iron/SystemF2Effect/Step/TfJudge.v
@@ -4,26 +4,31 @@ Require Export Iron.SystemF2Effect.Step.Frame.
 Require Export Iron.SystemF2Effect.Store.
 
 
+(******************************************************************************)
 (* Type of a frame stack.
    The frame stack is like a continuation that takes an expression of a certain
    type and produces a new expression. *)
-Inductive TYPEF : kienv -> tyenv -> stenv -> stack -> ty -> ty -> ty -> Prop := 
+Inductive
+ TYPEF :  kienv -> tyenv 
+       -> stenv -> stprops 
+       -> stack -> ty -> ty 
+       -> ty -> Prop := 
  | TfNil 
-   :  forall ke te se t
-   ,  TYPEF  ke te se nil t t (TBot KEffect)
+   :  forall ke te se sp t
+   ,  TYPEF  ke te se sp nil t t (TBot KEffect)
 
  | TfConsLet
-   :  forall ke te se fs sp t1 x2 t2 e2 t3 e3
-   ,  STOREP sp fs      (** WRONG, sp does not need to match fs *)
-   -> TYPEX  ke (te :> t1) se sp                 x2 t2 e2
-   -> TYPEF  ke te         se fs                 t2 t3 e3
-   -> TYPEF  ke te         se (fs :> FLet t1 x2) t1 t3 (TSum e2 e3)
+   :  forall ke te se sp fs t1 x2 t2 e2 t3 e3
+   ,  STOREP sp fs
+   -> TYPEX  ke (te :> t1) se sp                    x2 t2 e2
+   -> TYPEF  ke te         se sp fs                 t2 t3 e3
+   -> TYPEF  ke te         se sp (fs :> FLet t1 x2) t1 t3 (TSum e2 e3)
 
  | TfConsUse
-   :  forall ke te se fs t1 t2 e2 n
+   :  forall ke te se sp fs t1 t2 e2 n
    ,  not (In (FUse n) fs)
-   -> TYPEF  ke te se  fs                t1 t2 e2
-   -> TYPEF  ke te se (fs :> FUse n)     t1 t2 e2.
+   -> TYPEF  ke te se  sp fs             t1 t2 e2
+   -> TYPEF  ke te se  sp (fs :> FUse n) t1 t2 e2.
 
 Hint Constructors TYPEF.
 
@@ -32,12 +37,32 @@ Hint Constructors TYPEF.
 Ltac inverts_typef :=
  repeat 
   (try (match goal with 
-        | [ H: TYPEF _ _ _ (_ :> FLet _ _) _ _ _ |- _ ] => inverts H
-        | [ H: TYPEF _ _ _ (_ :> FUse _)   _ _ _ |- _ ] => inverts H
+        | [ H: TYPEF _ _ _ _ (_ :> FLet _ _) _ _ _ |- _ ] => inverts H
+        | [ H: TYPEF _ _ _ _ (_ :> FUse _)   _ _ _ |- _ ] => inverts H
         end);
    try inverts_type).
 
 
+Lemma typef_kind_effect
+ :  forall ke te se sp fs t1 t2 e
+ ,  TYPEF  ke te se sp fs t1 t2 e
+ -> KIND   ke sp e KEffect.
+Proof.
+ intros.
+ induction H; eauto.
+Qed.
+Hint Resolve typef_kind_effect.
+
+
+Lemma typef_kind_wfT
+ :  forall ke te se sp fs t1 t2 e
+ ,  TYPEF  ke te se sp fs t1 t2 e
+ -> wfT (length ke) e.
+Proof. eauto. Qed.
+Hint Resolve typef_kind_wfT.
+
+
+(*****************************************************************************)
 (* Type of an expression in a frame context. *)
 Inductive TYPEC 
    :  kienv -> tyenv 
@@ -46,9 +71,9 @@ Inductive TYPEC
    -> ty    -> ty -> Prop :=
  | TcExp
    :  forall ke te se sp fs x1 t1 e1 t2 e2 e3
-   ,  EquivT (TSum e1 e2) e3
+   ,  EquivT KEffect (TSum e1 e2) e3
    -> TYPEX  ke te se sp x1 t1 e1
-   -> TYPEF  ke te se fs t1 t2 e2
+   -> TYPEF  ke te se sp fs t1 t2 e2
    -> TYPEC  ke te se sp fs x1 t2 e3.
 
 Hint Constructors TYPEC.
@@ -62,7 +87,17 @@ Ltac inverts_typec :=
    try inverts_typef).
 
 
+Lemma typec_kind_effect
+ :  forall ke te se sp fs x t e
+ ,  TYPEC  ke te se sp fs x t e
+ -> KIND   ke sp e KEffect.
+Proof.
+ intros.
+ induction H; eauto.
+  admit.                   (* TODO: need kind trans under EquivT *)
+Qed.
 
-  
-   
+
+
+
 
