devel/Iron/SystemF2Effect/Type/EquivT.v
@@ -1,46 +1,47 @@
 
 Require Export Iron.SystemF2Effect.Type.Exp.Base.
+Require Export Iron.SystemF2Effect.Type.KiJudge.
 
 
 (* Type equivalence.
    The interesting cases all concern sums. *)
-Inductive EquivT : ty -> ty -> Prop :=
+Inductive EquivT : ki -> ty -> ty -> Prop :=
  | EqRefl
-   :  forall t
-   ,  EquivT t t
+   :  forall k t
+   ,  EquivT k t t
 
  | EqSym
-   :  forall t1 t2
-   ,  EquivT t1 t2 -> EquivT t2 t1
+   :  forall k t1 t2
+   ,  EquivT k t1 t2 -> EquivT k t2 t1
 
  | EqTrans
-   :  forall t1 t2 t3
-   ,  EquivT t1 t2 -> EquivT t2 t3
-   -> EquivT t1 t3
+   :  forall k t1 t2 t3
+   ,  EquivT k t1 t2 -> EquivT k t2 t3
+   -> EquivT k t1 t3
 
  | EqSumBot
-   : forall t k
-   , EquivT t             (TSum t (TBot k))
+   : forall k t
+   , EquivT k t             (TSum t (TBot k))
 
  | EqSumIdemp
-   : forall t
-   , EquivT t             (TSum t t)
+   : forall k t
+   , EquivT k t             (TSum t t)
 
  | EqSumComm
-   : forall t1 t2
-   , EquivT (TSum t1 t2)  (TSum t2 t1)
+   : forall k t1 t2
+   , EquivT k (TSum t1 t2)  (TSum t2 t1)
 
  | EqSumAssoc
-   : forall t1 t2 t3
-   , EquivT (TSum t1 (TSum t2 t3))
-            (TSum (TSum t1 t2) t3).
+   : forall k t1 t2 t3
+   , EquivT k (TSum t1 (TSum t2 t3))
+              (TSum (TSum t1 t2) t3).
 
 Hint Constructors EquivT.
 
 
 Lemma equivT_sum_left
  :  forall t k
- ,  EquivT t (TSum (TBot k) t).
+ ,  EquivT k t (TSum (TBot k) t).
 Proof.
  intros.
  eapply EqTrans.
@@ -48,3 +49,14 @@ Proof.
   eauto.
 Qed.
 Hint Resolve equivT_sum_left.
+
+
+Lemma equivT_kind
+ :  forall ke sp t1 t2 k
+ ,  EquivT k t1 t2
+ -> KIND   ke sp t1 k
+ -> KIND   ke sp t2 k.
+Proof.
+ admit.      (* Broken, will need to add KIND judge to EqRefl *)
+Qed. 
+
