devel/Iron/SystemF2Effect/Type/SubsT.v
@@ -5,69 +5,69 @@ Require Export Iron.SystemF2Effect.Type.EquivT.
 
 (* Type subsumptinon.
    The interesting cases all concern sums. *)
-Inductive SubsT : ty -> ty -> Prop :=
+Inductive SubsT : ki -> ty -> ty -> Prop :=
  | SbEquiv
-   :  forall t1 t2
-   ,  EquivT t1 t2
-   -> SubsT  t1 t2
+   :  forall k t1 t2
+   ,  EquivT k t1 t2
+   -> SubsT  k t1 t2
 
  | SbTrans
-   :  forall t1 t2 t3
-   ,  SubsT  t1 t2 -> SubsT t2 t3
-   -> SubsT  t1 t3
+   :  forall k t1 t2 t3
+   ,  SubsT  k t1 t2 -> SubsT k t2 t3
+   -> SubsT  k t1 t3
 
  | SbBot
-   :  forall t k
-   ,  SubsT  t (TBot k)
+   :  forall k t
+   ,  SubsT  k t (TBot k)
 
  | SbSumAbove
-   :  forall t1 t2 t3
-   ,  SubsT t1 t2
-   -> SubsT t1 t3
-   -> SubsT t1 (TSum t2 t3)
+   :  forall k t1 t2 t3
+   ,  SubsT  k t1 t2
+   -> SubsT  k t1 t3
+   -> SubsT  k t1 (TSum t2 t3)
 
  | SbSumBelow
-   :  forall t1 t2 t3
-   ,  SubsT t1 t2
-   -> SubsT (TSum t1 t3) t2.
+   :  forall k t1 t2 t3
+   ,  SubsT  k t1 t2
+   -> SubsT  k (TSum t1 t3) t2.
 
 Hint Constructors SubsT.
 
 
 Lemma substT_equiv_above
- :  forall t1 t1' t2
- ,  EquivT t1 t1' 
- -> SubsT  t1 t2  -> SubsT t1' t2.
+ :  forall k t1 t1' t2
+ ,  EquivT k t1 t1' 
+ -> SubsT  k t1 t2  -> SubsT k t1' t2.
 Proof. eauto. Qed.
 
 
 Lemma substT_equiv_below
- :  forall t1 t2 t2'
- ,  EquivT t2 t2' 
- -> SubsT  t1 t2  -> SubsT t1 t2'.
+ :  forall k t1 t2 t2'
+ ,  EquivT k t2 t2' 
+ -> SubsT  k t1 t2  -> SubsT k t1 t2'.
 Proof. eauto. Qed.
 
 
 Lemma subsT_sum_comm_below
- :  forall t1 t2 t3
- ,  SubsT t1 (TSum t2 t3)
- -> SubsT t1 (TSum t3 t2).
+ :  forall k t1 t2 t3
+ ,  SubsT  k t1 (TSum t2 t3)
+ -> SubsT  k t1 (TSum t3 t2).
 Proof. eauto. Qed.
 Hint Resolve subsT_sum_comm_below.
 
 
 Lemma subsT_sum_comm_above
- :  forall t1 t2 t3
- ,  SubsT (TSum t1 t2) t3
- -> SubsT (TSum t2 t1) t3.
+ :  forall k t1 t2 t3
+ ,  SubsT  k (TSum t1 t2) t3
+ -> SubsT  k (TSum t2 t1) t3.
 Proof. eauto. Qed.
 Hint Resolve subsT_sum_comm_above.
 
 
 Lemma subsT_sum_left
- : forall t1 t1' t2
- , SubsT  t1 t1'
--> SubsT (TSum t1 t2) (TSum t1' t2).
+ : forall k t1 t1' t2
+ , SubsT  k t1 t1'
+-> SubsT  k (TSum t1 t2) (TSum t1' t2).
 Proof.
  intros.
  eapply SbSumAbove. 
@@ -83,9 +83,9 @@ Hint Resolve subsT_sum_left.
 
 
 Lemma subsT_sum_right
- : forall t1 t2 t2'
- , SubsT  t2 t2'
--> SubsT (TSum t1 t2) (TSum t1 t2').
+ : forall k t1 t2 t2'
+ , SubsT  k t2 t2'
+-> SubsT  k (TSum t1 t2) (TSum t1 t2').
 Proof.
  intros.
  eapply SbSumAbove; eauto.
@@ -94,15 +94,14 @@ Hint Resolve subsT_sum_right.
 
 
 Lemma subsT_sum_merge
- :  forall t1 t1' t2 t2'
- ,  SubsT t1 t1'
- -> SubsT t2 t2'
- -> SubsT (TSum t1 t2) (TSum t1' t2').
+ :  forall k t1 t1' t2 t2'
+ ,  SubsT  k t1 t1'
+ -> SubsT  k t2 t2'
+ -> SubsT  k (TSum t1 t2) (TSum t1' t2').
 Proof.
  intros.
  eapply SbTrans.
   eapply subsT_sum_left.  eauto.
   eapply subsT_sum_right. eauto.
 Qed.
-
 
