devel/Iron/SystemF2Effect/Type/Operator/SubstTT/LemEquivT.v
@@ -4,9 +4,9 @@ Require Export Iron.SystemF2Effect.Type.EquivT.
 
 
 Lemma substTT_EquivT
- :  forall t1 t2 t3
- ,  EquivT t1 t2
- -> EquivT (substTT 0 t3 t1) (substTT 0 t3 t2).
+ :  forall k t1 t2 t3
+ ,  EquivT k t1 t2
+ -> EquivT k (substTT 0 t3 t1) (substTT 0 t3 t2).
 Proof.
  intros.
  induction H; snorm.
